Phase out static mutator code

src/MicroSail/Symbolic/Mutator.v
@@ -266,6 +266,9 @@ Module Mutators
 
   Definition EvarEnv (Σe Σr : Ctx (𝑺 * Ty)) : Type := Env (fun b => option (Term Σr (snd b))) Σe.
 
+  Global Instance SubstEvarEnv {Σe} : Subst (EvarEnv Σe) :=
+    fun Σ1 Σ2 ζ => env_map (fun _ => option_map (subst ζ)).
+
   Definition create_evarenv (Σe Σr : Ctx (𝑺 * Ty)) : EvarEnv Σe Σr :=
     env_tabulate (fun _ _ => None).
 
@@ -387,455 +390,6 @@ Module Mutators
 
   End WithEvarEnv.
 
-  Section MutatorResult.
-
-    (* Local Set Primitive Projections. *)
-    Local Set Maximal Implicit Insertion.
-
-    Record MutatorResult (Γ : Ctx (𝑿 * Ty)) (Σ : Ctx (𝑺 * Ty)) (A : Type) : Type :=
-      MkMutResult {
-          mutator_result_value : A;
-          mutator_result_state : SymbolicState Γ Σ;
-        }.
-
-  End MutatorResult.
-
-  Section Mutator.
-
-    Definition Mutator (Σ : Ctx (𝑺 * Ty)) (Γ1 Γ2 : Ctx (𝑿 * Ty)) (A : Type) : Type :=
-      SymbolicState Γ1 Σ -> Outcome (MutatorResult Γ2 Σ A).
-    Bind Scope mutator_scope with Mutator.
-
-    Definition mutator_demonic {Γ1 Γ2 I A Σ} (ms : I -> Mutator Σ Γ1 Γ2 A) : Mutator Σ Γ1 Γ2 A :=
-      fun (s : SymbolicState Γ1 Σ) => (⨂ i : I => ms i s)%out.
-    Definition mutator_angelic {Γ1 Γ2 I A Σ} (ms : I -> Mutator Σ Γ1 Γ2 A) : Mutator Σ Γ1 Γ2 A :=
-      fun (s : SymbolicState Γ1 Σ) => (⨁ i : I => ms i s)%out.
-    (* There are two kinds of failures of the symbolic execution. mutator_fail
-       is an unconditional fail: the current branch of choices is deemed invalid
-       and the executor should backtrack. mutator_contradiction is more liberal.
-       Instead of completely failing, it allows the current choices but requires
-       the path condition to be inconsistent. Essentially, this is should be a
-       mutator_block, but the execution engine could not derive the
-       inconsistency automatically. If in doubt, be more conservative and use
-       mutator_fail, because it allows for pruning of branches. Change to
-       mutator_contradiction if you're convinced that you require it for a
-       completeness issue. *)
-    Definition mutator_fail {Γ1 Γ2 A Σ} (msg : string) : Mutator Σ Γ1 Γ2 A :=
-      fun s => outcome_fail msg.
-    Definition mutator_contradiction {Γ1 Γ2 A Σ} (msg : string) : Mutator Σ Γ1 Γ2 A :=
-      fun s =>
-        (⨂ ι : SymInstance Σ =>
-         ⨂ _ : all_list (inst_formula ι) (symbolicstate_pathcondition s) =>
-         outcome_fail msg)%out.
-    Definition mutator_block {Γ1 Γ2 A Σ} : Mutator Σ Γ1 Γ2 A :=
-      fun s => outcome_block.
-
-    Definition mutator_demonic_binary {Γ1 Γ2 A Σ} (m1 m2 : Mutator Σ Γ1 Γ2 A) : Mutator Σ Γ1 Γ2 A :=
-      fun s => outcome_demonic_binary (m1 s) (m2 s).
-    Definition mutator_angelic_binary {Γ1 Γ2 A Σ} (m1 m2 : Mutator Σ Γ1 Γ2 A) : Mutator Σ Γ1 Γ2 A :=
-      fun s => outcome_angelic_binary (m1 s) (m2 s).
-
-    Definition mutator_pure {Γ A Σ} (a : A) : Mutator Σ Γ Γ A :=
-      fun s => outcome_pure (MkMutResult a s).
-    Definition mutator_bind {Γ1 Γ2 Γ3 A B Σ} (ma : Mutator Σ Γ1 Γ2 A) (f : A -> Mutator Σ Γ2 Γ3 B) : Mutator Σ Γ1 Γ3 B :=
-      fun s0 => outcome_bind (ma s0) (fun '(MkMutResult a s1) => outcome_bind (f a s1) (fun '(MkMutResult b s2) => outcome_pure (MkMutResult b s2))).
-    Definition mutator_bind_right {Γ1 Γ2 Γ3 A B Σ} (ma : Mutator Σ Γ1 Γ2 A) (mb : Mutator Σ Γ2 Γ3 B) : Mutator Σ Γ1 Γ3 B :=
-      mutator_bind ma (fun _ => mb).
-    Definition mutator_bind_left {Γ1 Γ2 Γ3 A B Σ} (ma : Mutator Σ Γ1 Γ2 A) (mb : Mutator Σ Γ2 Γ3 B) : Mutator Σ Γ1 Γ3 A :=
-      mutator_bind ma (fun a => mutator_bind mb (fun _ => mutator_pure a)).
-    Definition mutator_map {Γ1 Γ2 A B Σ} (f : A -> B) (ma : Mutator Σ Γ1 Γ2 A) : Mutator Σ Γ1 Γ2 B :=
-      mutator_bind ma (fun a => mutator_pure (f a)).
-    Definition mutator_angelic_list {Γ A Σ} (msg : string) :
-      list A -> Mutator Σ Γ Γ A :=
-      fix mutator_angelic_list (xs : list A) :=
-        match xs with
-        | []      => mutator_contradiction msg
-        | x :: [] => mutator_pure x
-        | x :: xs => mutator_angelic_binary (mutator_pure x) (mutator_angelic_list xs)
-        end.
-    Definition mutator_demonic_list {Γ A Σ} :
-      list A -> Mutator Σ Γ Γ A :=
-      fix mutator_demonic_list (xs : list A) :=
-        match xs with
-        | []      => mutator_block
-        | x :: [] => mutator_pure x
-        | x :: xs => mutator_demonic_binary (mutator_pure x) (mutator_demonic_list xs)
-        end.
-    Definition mutator_angelic_finite {Γ Σ} (msg : string) A `{finite.Finite A} :
-      Mutator Σ Γ Γ A := mutator_angelic_list msg (finite.enum A).
-    Definition mutator_demonic_finite {Γ Σ} A `{finite.Finite A} :
-      Mutator Σ Γ Γ A := mutator_demonic_list (finite.enum A).
-
-    Global Arguments mutator_bind {_ _ _ _ _ _} _ _ /.
-    Global Arguments mutator_bind_right {_ _ _ _ _ _} _ _ /.
-    Global Arguments mutator_angelic_finite {_ _} msg%string A {_ _} /.
-    Global Arguments mutator_demonic_finite {_ _} A {_ _} /.
-
-  End Mutator.
-  Bind Scope mutator_scope with Mutator.
-
-  Module MutatorNotations.
-
-    Notation "'⨂' x .. y => F" :=
-      (mutator_demonic (fun x => .. (mutator_demonic (fun y => F)) .. )) : mutator_scope.
-
-    Notation "'⨁' x .. y => F" :=
-      (mutator_angelic (fun x => .. (mutator_angelic (fun y => F)) .. )) : mutator_scope.
-
-    Infix "⊗" := mutator_demonic_binary (at level 40, left associativity) : mutator_scope.
-    Infix "⊕" := mutator_angelic_binary (at level 50, left associativity) : mutator_scope.
-
-    Notation "x <- ma ;; mb" :=
-      (mutator_bind ma (fun x => mb))
-        (at level 80, ma at level 90, mb at level 200, right associativity) : mutator_scope.
-    Notation "ma >>= f" := (mutator_bind ma f) (at level 50, left associativity) : mutator_scope.
-    Notation "m1 ;; m2" := (mutator_bind m1 (fun _ => m2)) : mutator_scope.
-    Notation "ma *> mb" := (mutator_bind_right ma mb) (at level 50, left associativity) : mutator_scope.
-    Notation "ma <* mb" := (mutator_bind_left ma mb) (at level 50, left associativity) : mutator_scope.
-
-  End MutatorNotations.
-  Import MutatorNotations.
-
-  Section MutatorOperations.
-
-    Local Open Scope mutator_scope.
-
-    Definition mutator_state {Γ Γ' Σ A} (f : SymbolicState Γ Σ -> (SymbolicState Γ' Σ * A)) : Mutator Σ Γ Γ' A :=
-      fun s => outcome_pure (let (s1,a) := f s in MkMutResult a s1).
-    Definition mutator_modify {Γ Γ' Σ} (f : SymbolicState Γ Σ -> SymbolicState Γ' Σ) : Mutator Σ Γ Γ' unit :=
-      mutator_state (fun s => (f s,tt)).
-    Definition mutator_put {Γ Γ' Σ} (s : SymbolicState Γ' Σ) : Mutator Σ Γ Γ' unit :=
-      mutator_state (fun _ => (s,tt)).
-    Definition mutator_get {Γ Σ} : Mutator Σ Γ Γ (SymbolicState Γ Σ) :=
-      mutator_state (fun s => (s,s)).
-
-    Definition mutator_state_local {Γ Γ' Σ A} (f : SymbolicLocalStore Γ Σ -> (SymbolicLocalStore Γ' Σ * A)) : Mutator Σ Γ Γ' A :=
-      mutator_state (fun '(MkSymbolicState Φ δ ĥ) => let (δ',a) := f δ in (MkSymbolicState Φ δ' ĥ,a)).
-    Definition mutator_modify_local {Γ Γ' Σ} (f : SymbolicLocalStore Γ Σ -> SymbolicLocalStore Γ' Σ) : Mutator Σ Γ Γ' unit :=
-      mutator_state_local (fun δ => (f δ,tt)).
-    Definition mutator_put_local {Γ Γ' Σ} (δ : SymbolicLocalStore Γ' Σ) : Mutator Σ Γ Γ' unit :=
-      mutator_state_local (fun _ => (δ,tt)).
-    Definition mutator_get_local {Γ Σ} : Mutator Σ Γ Γ (SymbolicLocalStore Γ Σ) :=
-      mutator_state_local (fun δ => (δ,δ)).
-    Definition mutator_gets_local {Γ Σ A} (f : SymbolicLocalStore Γ Σ -> A) : Mutator Σ Γ Γ A :=
-      mutator_state_local (fun δ => (δ,f δ)).
-    Definition mutator_pop_local {Γ x σ Σ} : Mutator Σ (Γ ▻ (x , σ)) Γ unit :=
-      mutator_modify_local (fun δ => env_tail δ).
-    Definition mutator_pops_local {Γ Σ} Δ : Mutator Σ (Γ ▻▻ Δ) Γ unit :=
-      mutator_modify_local (fun δΓΔ => env_drop Δ δΓΔ).
-    Definition mutator_push_local {Γ x σ Σ} (t : Term Σ σ) : Mutator Σ Γ (Γ ▻ (x , σ)) unit :=
-      mutator_modify_local (fun δ => env_snoc δ (x , σ) t).
-    Definition mutator_pushs_local {Γ Δ Σ} (δΔ : NamedEnv (Term Σ) Δ) : Mutator Σ Γ (Γ ▻▻ Δ) unit :=
-      mutator_modify_local (fun δΓ => env_cat δΓ δΔ).
-
-    Definition mutator_state_heap {Γ Σ A} (f : SymbolicHeap Σ -> (SymbolicHeap Σ * A)) : Mutator Σ Γ Γ A :=
-      mutator_state (fun '(MkSymbolicState Φ δ h) => let (h',a) := f h in (MkSymbolicState Φ δ h',a)).
-    Definition mutator_modify_heap {Γ Σ} (f : SymbolicHeap Σ -> SymbolicHeap Σ) : Mutator Σ Γ Γ unit :=
-      mutator_state_heap (fun h => (f h,tt)).
-    Definition mutator_get_heap {Γ Σ} : Mutator Σ Γ Γ (SymbolicHeap Σ) :=
-      mutator_state_heap (fun h => (h,h)).
-    Definition mutator_put_heap {Γ Σ} (h : SymbolicHeap Σ) : Mutator Σ Γ Γ unit :=
-      mutator_state_heap (fun _ => (h,tt)).
-
-    Definition mutator_state_pathcondition {Γ Σ A} (f : PathCondition Σ -> (PathCondition Σ * A)) : Mutator Σ Γ Γ A :=
-      mutator_state (fun '(MkSymbolicState Φ δ h) => let (Φ',a) := f Φ in (MkSymbolicState Φ' δ h,a)).
-    Definition mutator_modify_pathcondition {Γ Σ} (f : PathCondition Σ -> PathCondition Σ) : Mutator Σ Γ Γ unit :=
-      mutator_state_pathcondition (fun Φ => (f Φ,tt)).
-    Definition mutator_get_pathcondition {Γ Σ} : Mutator Σ Γ Γ (PathCondition Σ) :=
-      mutator_state_pathcondition (fun Φ => (Φ,Φ)).
-    Definition mutator_put_pathcondition {Γ Σ} (Φ : PathCondition Σ) : Mutator Σ Γ Γ unit :=
-      mutator_state_pathcondition (fun _ => (Φ,tt)).
-
-    Definition mutator_eval_exp {Γ σ Σ} (e : Exp Γ σ) : Mutator Σ Γ Γ (Term Σ σ) :=
-      mutator_gets_local (fun δ => symbolic_eval_exp δ e).
-    Definition mutator_eval_exps {Γ Σ} {σs : Ctx (𝑿 * Ty)} (es : NamedEnv (Exp Γ) σs) : Mutator Σ Γ Γ (NamedEnv (Term Σ) σs) :=
-      mutator_gets_local (fun δ => env_map (fun _ => symbolic_eval_exp δ) es).
-
-    Definition mutator_assume_formula {Γ Σ} (fml : Formula Σ) : Mutator Σ Γ Γ unit :=
-      match try_solve_formula fml with
-      | Some true  => mutator_pure tt
-      | Some false => mutator_block
-      | None       => mutator_modify (symbolic_assume_formula fml)
-      end.
-    (* Definition mutator_assume_formula {Γ Σ} (fml : Formula Σ) : Mutator Σ Γ Γ unit := *)
-    (*   mutator_modify (symbolic_assume_formula fml). *)
-    Definition mutator_assume_term {Γ Σ} (t : Term Σ ty_bool) : Mutator Σ Γ Γ unit :=
-      mutator_assume_formula (formula_bool t).
-    Definition mutator_assume_exp {Γ Σ} (e : Exp Γ ty_bool) : Mutator Σ Γ Γ unit :=
-      mutator_eval_exp e >>= mutator_assume_term.
-
-    Definition mutator_assert_formula {Γ Σ} (fml : Formula Σ) : Mutator Σ Γ Γ unit :=
-      match try_solve_formula fml with
-      | Some true  => mutator_pure tt
-      | Some false => mutator_fail "Err [mutator_assert_formula]: unsatisfiable"
-      | None       => fun δ =>
-                        outcome_assertk
-                          (valid_obligation (obligation (symbolicstate_pathcondition δ) fml))
-                          (outcome_pure (MkMutResult tt δ))
-      end.
-    Definition mutator_assert_formulas {Γ Σ} (fmls : list (Formula Σ)) : Mutator Σ Γ Γ unit :=
-      fold_right (fun fml m => mutator_assert_formula fml ;; m) (mutator_pure tt) fmls.
-    (* Definition mutator_assert_formula {Γ Σ} (fml : Formula Σ) : Mutator Σ Γ Γ unit := *)
-    (*   fun δ => outcome_pure (tt , δ , obligation (symbolicstate_pathcondition δ) fml :: nil). *)
-
-    Definition mutator_assert_term {Γ Σ} (t : Term Σ ty_bool) : Mutator Σ Γ Γ unit :=
-      mutator_assert_formula (formula_bool t).
-    Definition mutator_assert_exp {Γ Σ} (e : Exp Γ ty_bool) : Mutator Σ Γ Γ unit :=
-      mutator_eval_exp e >>= mutator_assert_term.
-
-    Definition mutator_produce_chunk {Γ Σ} (c : Chunk Σ) : Mutator Σ Γ Γ unit :=
-      mutator_modify_heap (fun h => c :: h).
-
-    Definition mutator_consume_chunk {Γ Σ} (c : Chunk Σ) : Mutator Σ Γ Γ unit :=
-      mutator_get_heap >>= fun h =>
-      mutator_get_pathcondition >>= fun pc =>
-      mutator_angelic_list
-        "Err [mutator_consume_chunk]: empty extraction"
-        (extract_chunk_eqb c h pc) >>= fun '(pc' , h') =>
-        mutator_put_heap h' ;;
-        mutator_put_pathcondition pc'.
-
-    Global Arguments mutator_push_local {Γ _ _} [Σ] _.
-    Global Arguments mutator_assume_formula {Γ} [Σ] _.
-    Global Arguments mutator_assume_term {Γ} [Σ] _.
-    Global Arguments mutator_assert_formula {Γ} [Σ] _.
-    Global Arguments mutator_assert_formulas {Γ} [Σ] _.
-    Global Arguments mutator_produce_chunk {Γ} [Σ] _.
-    Global Arguments mutator_consume_chunk {Γ} [Σ] _.
-
-    Fixpoint mutator_produce {Γ Σ Σ'} (ζ : Sub Σ Σ') (asn : Assertion Σ) : Mutator Σ' Γ Γ unit :=
-      match asn with
-      | asn_bool b      => mutator_assume_term (sub_term ζ b)
-      | asn_prop P      => mutator_assume_formula (formula_prop ζ P)
-      | asn_eq t1 t2    => mutator_assume_formula (formula_eq (sub_term ζ t1) (sub_term ζ t2))
-      | asn_chunk c     => mutator_produce_chunk (sub_chunk ζ c)
-      | asn_if b a1 a2  => (mutator_assume_term (sub_term ζ b)            *> mutator_produce ζ a1) ⊗
-                           (mutator_assume_term (sub_term ζ (term_not b)) *> mutator_produce ζ a2)
-      | @asn_match_enum _ E k1 alts =>
-        k2 <- mutator_demonic_finite (𝑬𝑲 E) ;;
-        mutator_assume_formula
-          (formula_eq (sub_term ζ k1) (term_enum E k2)) ;;
-        mutator_produce ζ (alts k2)
-      | asn_sep a1 a2   => mutator_produce ζ a1 *> mutator_produce ζ a2
-      | asn_exist ς τ a => mutator_fail
-                             "Err [mutator_produce]: case [asn_exist] not implemented"
-      end.
-
-    Section MutatorConsumeEvar.
-      Context {Σr : Ctx (𝑺 * Ty)} {Γ : Ctx (𝑿 * Ty)}.
-
-      Definition mutator_consume_chunk_evar {Σe} (c : Chunk Σe) (L : EvarEnv Σe Σr) : Mutator Σr Γ Γ (EvarEnv Σe Σr) :=
-        mutator_get_heap >>= fun h =>
-        mutator_angelic_list
-          "Err [mutator_consume_chunk_evar]: empty extraction"
-          (extract_chunk c h L) >>= fun '(L' , h') =>
-        mutator_put_heap h' *> mutator_pure L'.
-
-      Fixpoint mutator_consume_evar {Σe} (asn : Assertion Σe) (L : EvarEnv Σe Σr) : Mutator Σr Γ Γ (EvarEnv Σe Σr) :=
-        match asn with
-        | asn_bool tb =>
-          match eval_term_evar L tb with
-          | Some tb' => mutator_assert_term tb' *> mutator_pure L
-          | None     => mutator_fail "Err [mutator_consume_evar]: uninstantiated variables when consuming bool assertion"
-          end
-        | asn_prop P =>
-          match evarenv_to_option_sub L with
-          | Some ζ => mutator_assert_formula (formula_prop ζ P) *> mutator_pure L
-          | None   => mutator_fail "Err [mutator_consume_evar]: uninstantiated variables when consuming prop assertion"
-          end
-        | asn_eq t1 t2 =>
-          match eval_term_evar L t1, eval_term_evar L t2 with
-          | Some t1', Some t2' =>
-            mutator_assert_formula (formula_eq t1' t2') *> mutator_pure L
-          | _, _ => mutator_fail "Err [mutator_consume_evar]: uninstantiated variables when consuming equality assertion"
-                              end
-        | asn_chunk c => mutator_consume_chunk_evar c L
-        | asn_if tb a1 a2 =>
-          match eval_term_evar L tb with
-          | Some tb' => (mutator_assume_term tb'            *> mutator_consume_evar a1 L) ⊗
-                        (mutator_assume_term (term_not tb') *> mutator_consume_evar a2 L)
-          | None     => mutator_fail "Err [mutator_consume_evar]: uninstantiated variables when consuming if assertion"
-          end
-        | @asn_match_enum _ E k1 alts =>
-          match eval_term_evar L k1 with
-          | Some k1' => ⨁ k2 : 𝑬𝑲 E =>
-            mutator_assert_formula (formula_eq k1' (term_enum E k2)) ;;
-            mutator_consume_evar (alts k2) L
-          | None => mutator_fail "Err [mutator_consume_evar]: uninstantiated variables when consuming match enum assertion"
-          end
-        | asn_sep a1 a2 => mutator_consume_evar a1 L >>= mutator_consume_evar a2
-        | asn_exist ς τ a =>
-          mutator_consume_evar a (env_snoc L _ None) >>= fun La' =>
-          match env_unsnoc La' with
-          | (L', Some a) => mutator_pure L'
-          | _            => mutator_fail "Err [mutator_consume_evar]: uninstantiated existential variable"
-          end
-        end.
-
-      Definition mutator_assert_term_eq_evar {Σe σ} (te : Term Σe σ) (tr : Term Σr σ) (L : EvarEnv Σe Σr) : Mutator Σr Γ Γ (EvarEnv Σe Σr) :=
-        match match_term te tr L with
-        | Some L' => mutator_pure L'
-        | None    => match eval_term_evar L te with
-                     | Some te' => mutator_assert_formula (formula_eq te' tr) *> mutator_pure L
-                     | None     => mutator_fail "Err [mutator_consume_evar]: uninstantiated existential variable"
-                     end
-        end.
-
-      Equations(noeqns) mutator_assert_namedenv_eq_evar {X Σe σs} (te : NamedEnv (X:=X) (Term Σe) σs) (tr : NamedEnv (Term Σr) σs) :
-        EvarEnv Σe Σr -> Mutator Σr Γ Γ (EvarEnv Σe Σr) :=
-        mutator_assert_namedenv_eq_evar env_nil env_nil := mutator_pure;
-        mutator_assert_namedenv_eq_evar (env_snoc E1 b1 t1) (env_snoc E2 b2 t2) :=
-          fun L => mutator_assert_namedenv_eq_evar E1 E2 L >>= mutator_assert_term_eq_evar t1 t2.
-
-    End MutatorConsumeEvar.
-
-    Fixpoint mutator_consume {Γ Σ Σ'} (ζ : Sub Σ Σ') (asn : Assertion Σ) : Mutator Σ' Γ Γ unit :=
-      match asn with
-      | asn_bool b      => mutator_assert_term (sub_term ζ b)
-      | asn_prop P      => mutator_assert_formula (formula_prop ζ P)
-      | asn_eq t1 t2    => mutator_assert_formula (formula_eq (sub_term ζ t1) (sub_term ζ t2))
-      | asn_chunk c     => mutator_consume_chunk (sub_chunk ζ c)
-      | asn_if b a1 a2  => (mutator_assume_term (sub_term ζ b)            *> mutator_consume ζ a1) ⊗
-                           (mutator_assume_term (sub_term ζ (term_not b)) *> mutator_consume ζ a2)
-      | @asn_match_enum _ E k1 alts =>
-        k2 <- mutator_angelic_finite
-                "Err [mutator_consume]: case asn_match_enum failed"
-                (𝑬𝑲 E) ;;
-        mutator_assert_formula
-          (formula_eq (sub_term ζ k1) (term_enum E k2)) ;;
-        mutator_consume ζ (alts k2)
-      | asn_sep a1 a2   => mutator_consume ζ a1 *> mutator_consume ζ a2
-      | asn_exist ς τ a => ⨁ t : Term Σ' τ => mutator_consume (sub_snoc ζ (ς , τ) t) a
-      end.
-
-    Section WithCont.
-      Context {Γ Σ E R} (cont : forall K : 𝑬𝑲 E, Mutator Σ Γ Γ R).
-
-      Equations(noeqns) mutator_exec_match_enum (t : Term Σ (ty_enum E)) : Mutator Σ Γ Γ R :=
-        mutator_exec_match_enum (term_lit _ l) := cont l;
-        mutator_exec_match_enum t :=
-          K <- mutator_demonic_finite (𝑬𝑲 E) ;;
-          mutator_assume_formula (formula_eq t (term_lit (ty_enum E) K)) ;;
-          cont K.
-
-    End WithCont.
-
-    (* TODO: The code should be rewritten so this variable can be removed. *)
-    Parameter dummy : 𝑺.
-
-    (* Definition mutator_call {Σ Γ Δ τ} (contract : SepContract Δ τ) (ts : NamedEnv (Term Σ) Δ) : Mutator Σ Γ Γ (Term Σ τ) := *)
-    (*   match contract with *)
-    (*   (* | @sep_contract_unit _ Σe δ req ens => *) *)
-    (*   (*   mutator_consume_evar req (create_evarenv Σe Σ) >>= fun L1 => *) *)
-    (*   (*   mutator_assert_namedenv_eq_evar δ ts L1 >>= fun L2 => *) *)
-    (*   (*   match ghost_env_to_option_sub L2 with *) *)
-    (*   (*   | Some ζ => mutator_produce ζ ens *> *) *)
-    (*   (*               mutator_pure (term_lit ty_unit tt) *) *)
-    (*   (*   | None   => mutator_fail "Err [mutator_exec]: uninstantiated variables after consuming precondition" *) *)
-    (*   (*   end *) *)
-    (*   | @sep_contract_result_pure _ _ Σe δ result req ens => *)
-    (*     mutator_consume_evar req (create_evar_env Σe Σ) >>= fun L1 => *)
-    (*     mutator_assert_namedenv_eq_evar δ ts L1 >>= fun L2 => *)
-    (*     match ghost_env_to_option_sub L2 with *)
-    (*     | Some ζ => mutator_produce ζ ens *> *)
-    (*                 mutator_pure (sub_term ζ result) *)
-    (*     | None   => mutator_contradiction "Err [mutator_exec]: uninstantiated variables after consuming precondition" *)
-    (*     end *)
-    (*   | @sep_contract_result _ _ Σ' δ result req ens => mutator_fail "Err [mutator_exec]: stm_call of sep_contract_none_result function not implemented" *)
-    (*   | sep_contract_none _ _ => mutator_fail "Err [mutator_exec]: stm_call of sep_contract_none function" *)
-    (*   end. *)
-
-    Fixpoint mutator_exec {Σ Γ τ} (s : Stm Γ τ) : Mutator Σ Γ Γ (Term Σ τ) :=
-      match s with
-      | stm_lit _ l => mutator_pure (term_lit τ l)
-      | stm_exp e => mutator_eval_exp e
-      | stm_let x τ s k =>
-        mutator_exec s >>= fun v =>
-        mutator_push_local v *>
-        mutator_exec k              <*
-        mutator_pop_local
-      | stm_block δ k =>
-        mutator_pushs_local (lift δ) *>
-        mutator_exec k <*
-        mutator_pops_local _
-      | stm_assign x e => mutator_exec e >>= fun v =>
-        mutator_modify_local (fun δ => δ ⟪ x ↦ v ⟫)%env *>
-        mutator_pure v
-      | stm_call f es => mutator_fail "Err [mutator_exec]: stm_call not supported"
-      | stm_call_external f es => mutator_fail "Err [mutator_exec]: stm_call not supported"
-      | stm_call_frame δ' s =>
-        δ <- mutator_get_local ;;
-        mutator_put_local (lift δ') ;;
-        t <- mutator_exec s ;;
-        mutator_put_local δ ;;
-        mutator_pure t
-      | stm_if e s1 s2 =>
-        (mutator_assume_exp e ;; mutator_exec s1) ⊗
-        (mutator_assume_exp (exp_not e) ;; mutator_exec s2)
-      | stm_seq e k => mutator_exec e ;; mutator_exec k
-      | stm_assertk e1 _ k =>
-        t <- mutator_eval_exp e1 ;;
-        mutator_assert_term t ;;
-        mutator_exec k
-      | stm_fail _ s => mutator_block
-      | stm_match_enum E e alts =>
-        mutator_eval_exp e >>=
-        mutator_exec_match_enum (fun K => mutator_exec (alts K))
-      | stm_read_register reg =>
-        mutator_consume_chunk_evar (chunk_ptsreg reg (@term_var _ dummy τ inctx_zero)) [None]%arg >>= fun L =>
-        match env_unsnoc L with
-        | (_ , Some t) => mutator_produce_chunk (chunk_ptsreg reg t) *>
-                          mutator_pure t
-        (* Extracting the points to chunk should never fail here. Because there is exactly one binding
-           in the ghost environment and the chunk matching will always instantiate it. *)
-        | _            => mutator_fail "Err [mutator_exec]: You have found a unicorn."
-        end
-      | stm_write_register reg e =>
-        mutator_eval_exp e >>= fun v =>
-        mutator_consume_chunk_evar (chunk_ptsreg reg (@term_var _ dummy τ inctx_zero)) [None]%arg ;;
-        mutator_produce_chunk (chunk_ptsreg reg v) *>
-        mutator_pure v
-      | stm_match_list e alt_nil xh xt alt_cons =>
-        mutator_fail "Err [mutator_exec]: stm_match_list not supported. use dynamic mutators"
-      | stm_match_sum e xinl alt_inl xinr alt_inr =>
-        mutator_fail "Err [mutator_exec]: stm_match_sum not supported. use dynamic mutators"
-      | stm_match_pair e xl xr rhs =>
-        mutator_fail "Err [mutator_exec]: stm_match_pair not supported. use dynamic mutators"
-      | stm_match_tuple e p rhs =>
-        mutator_fail "Err [mutator_exec]: stm_match_tuple not supported. use dynamic mutators"
-      | stm_match_union U e alt__pat alt__rhs =>
-        mutator_fail "Err [mutator_exec]: stm_match_union not supported. use dynamic mutators"
-      | stm_match_record R e p rhs =>
-        mutator_fail "Err [mutator_exec]: stm_match_record not supported. use dynamic mutators"
-      | stm_bind s k => mutator_fail "Err [mutator_exec]: stm_bind not supported"
-      end.
-
-    Definition mutator_leakcheck {Γ Σ} : Mutator Σ Γ Γ unit :=
-      mutator_get_heap >>= fun h =>
-      match h with
-      | nil => mutator_pure tt
-      | _   => mutator_fail "Err [mutator_leakcheck]: heap leak"
-      end.
-
-  End MutatorOperations.
-
-  Definition mutator_outcome_contract {Δ : Ctx (𝑿 * Ty)} {τ : Ty} (c : SepContract Δ τ) :
-    Stm Δ τ -> Outcome unit :=
-    match c with
-    | MkSepContract _ _ Σe δ req result ens =>
-      fun s =>
-        let mut := (mutator_produce (sub_id Σe) req ;;
-                    mutator_exec s >>= fun v =>
-                    mutator_consume (env_snoc (sub_id Σe) (result,τ) v) ens;;
-                    mutator_leakcheck)%mut in
-        let out := mut (symbolicstate_initial δ) in
-        outcome_map (fun _ => tt) out
-    end.
-
-  Definition ValidContractMut (Δ : Ctx (𝑿 * Ty)) (τ : Ty)
-             (c : SepContract Δ τ) (body : Stm Δ τ) : Prop :=
-    outcome_safe (mutator_outcome_contract c body).
-
   Section DynamicMutatorResult.
 
     (* Local Set Primitive Projections. *)
@@ -845,10 +399,11 @@ Module Mutators
       MkDynMutResult {
           dmutres_context      : Ctx (𝑺 * Ty);
           dmutres_substitution : Sub Σ dmutres_context;
-          dmutres_result       : MutatorResult Γ dmutres_context (A dmutres_context);
+          dmutres_result_value : A dmutres_context;
+          dmutres_result_state : SymbolicState Γ dmutres_context;
         }.
 
-    Global Arguments MkDynMutResult {_ _ _ _} _ _.
+    Global Arguments MkDynMutResult {_ _ _ _} _ _ _.
 
   End DynamicMutatorResult.
 
@@ -863,13 +418,13 @@ Module Mutators
     Bind Scope dmut_scope with DynamicMutator.
 
     Definition dmut_pure {Γ A} `{Subst A} {Σ} (a : A Σ) : DynamicMutator Γ Γ A Σ :=
-      fun Σ' ζ s => outcome_pure (MkDynMutResult (sub_id Σ') (MkMutResult (subst ζ a) s)).
+      fun Σ' ζ s => outcome_pure (MkDynMutResult (sub_id Σ') (subst ζ a) s).
     Definition dmut_bind {Γ1 Γ2 Γ3 A B Σ}
       (ma : DynamicMutator Γ1 Γ2 A Σ) (f : forall Σ', Sub Σ Σ' -> A Σ' -> DynamicMutator Γ2 Γ3 B Σ') : DynamicMutator Γ1 Γ3 B Σ :=
       fun Σ0 ζ0 s0 =>
-        outcome_bind (ma Σ0 ζ0 s0)                            (fun '(MkDynMutResult ζ1 (MkMutResult a s1)) =>
-        outcome_bind (f _ (sub_comp ζ0 ζ1) a _ (sub_id _) s1) (fun '(MkDynMutResult ζ2 (MkMutResult b s2)) =>
-        outcome_pure (MkDynMutResult (sub_comp ζ1 ζ2) (MkMutResult b s2)))).
+        outcome_bind (ma Σ0 ζ0 s0)                            (fun '(MkDynMutResult ζ1 a s1) =>
+        outcome_bind (f _ (sub_comp ζ0 ζ1) a _ (sub_id _) s1) (fun '(MkDynMutResult ζ2 b s2) =>
+        outcome_pure (MkDynMutResult (sub_comp ζ1 ζ2) b s2))).
     Definition dmut_join {Γ1 Γ2 Γ3 A Σ} (mm : DynamicMutator Γ1 Γ2 (DynamicMutator Γ2 Γ3 A) Σ) :
       DynamicMutator Γ1 Γ3 A Σ := dmut_bind mm (fun _ _ m => m).
 
@@ -897,17 +452,25 @@ Module Mutators
       DynamicMutator Γ1 Γ3 (fun Σ => A Σ * B Σ)%type Σ :=
       dmut_fmap2 ma mb (fun _ _ => pair).
 
-    Definition dmut_lift {Γ1 Γ2 A} {Σ} (m : forall Σ', Sub Σ Σ' -> Mutator Σ' Γ1 Γ2 (A Σ')) : DynamicMutator Γ1 Γ2 A Σ :=
-      fun Σ1 ζ1 s => outcome_map (MkDynMutResult (sub_id _)) (m Σ1 ζ1 s).
-    Definition dmut_lift_kleisli {Γ1 Γ2 A B} `{Subst A} (m : forall Σ, A Σ -> Mutator Σ Γ1 Γ2 (B Σ)) :
-      forall Σ, A Σ -> DynamicMutator Γ1 Γ2 B Σ :=
-      fun _ a => dmut_lift (fun _ ζ => m _ (subst ζ a)).
+    (* There are two kinds of failures of the symbolic execution. dmut_fail
+       is an unconditional fail: the current branch of choices is deemed invalid
+       and the executor should backtrack. dmut_contradiction is more liberal.
+       Instead of completely failing, it allows the current choices but requires
+       the path condition to be inconsistent. Essentially, this is should be a
+       dmut_block, but the execution engine could not derive the
+       inconsistency automatically. If in doubt, be more conservative and use
+       dmut_fail, because it allows for pruning of branches. Change to
+       dmut_contradiction if you're convinced that you require it for a
+       completeness issue. *)
     Definition dmut_fail {Γ1 Γ2 A Σ} (msg : string) : DynamicMutator Γ1 Γ2 A Σ :=
-      dmut_lift (fun _ _ => mutator_fail msg).
+      fun _ _ _ => outcome_fail msg.
     Definition dmut_contradiction {Γ1 Γ2 A Σ} (msg : string) : DynamicMutator Γ1 Γ2 A Σ :=
-      dmut_lift (fun _ _ => mutator_contradiction msg).
+      fun Σ1 ζ1 s1 =>
+        (⨂ (ι : SymInstance Σ1)
+            (_ : all_list (inst_formula ι) (symbolicstate_pathcondition s1)) =>
+         outcome_fail msg)%out.
     Definition dmut_block {Γ1 Γ2 A Σ} : DynamicMutator Γ1 Γ2 A Σ :=
-      dmut_lift (fun _ _ => mutator_block).
+      fun _ _ _ => outcome_block.
 
     Definition dmut_angelic {Γ1 Γ2 I A Σ} (ms : I -> DynamicMutator Γ1 Γ2 A Σ) : DynamicMutator Γ1 Γ2 A Σ :=
       fun Σ1 ζ1 s1 => outcome_angelic (fun i => ms i Σ1 ζ1 s1).
@@ -948,7 +511,7 @@ Module Mutators
     Definition dmut_fresh {Γ A Σ} b (ma : DynamicMutator Γ Γ A (Σ ▻ b)) : DynamicMutator Γ Γ A Σ :=
       fun Σ1 ζ1 s1 =>
         outcome_map
-          (fun '(MkDynMutResult ζ r) => MkDynMutResult (sub_comp sub_wk1 ζ) r)
+          (fun '(MkDynMutResult ζ a s) => MkDynMutResult (sub_comp sub_wk1 ζ) a s)
           (ma _ (sub_up1 ζ1) (wk1 s1)).
     Global Arguments dmut_fresh {_ _ _} _ _.
     Definition dmut_freshtermvar {Γ Σ σ} (x : 𝑺) : DynamicMutator Γ Γ (fun Σ => Term Σ σ) Σ :=
@@ -957,66 +520,6 @@ Module Mutators
 
   End DynamicMutator.
   Bind Scope dmut_scope with DynamicMutator.
-
-  Module Proper.
-
-    Definition Mor (Σ : Ctx (𝑺 * Ty)) (A B : Ctx (𝑺 * Ty) -> Type) : Type :=
-      forall Σ', Sub Σ Σ' -> A Σ' -> B Σ'.
-
-    Definition DynamicMutator (Γ1 Γ2 : Ctx (𝑿 * Ty)) (A : Ctx (𝑺 * Ty) -> Type) (Σ : Ctx (𝑺 * Ty)) : Type :=
-      SymbolicState Γ1 Σ -> Outcome (DynamicMutatorResult Γ2 A Σ).
-
-    Definition dmut_pure {Γ A} {Σ} : Mor Σ A (DynamicMutator Γ Γ A) :=
-      fun Σ' ζ' a s =>
-        outcome_pure (MkDynMutResult (sub_id Σ') (MkMutResult a s)).
-    Definition dmut_map {Γ1 Γ2 A B Σ} (f : Mor Σ A B) : Mor Σ (DynamicMutator Γ1 Γ2 A) (DynamicMutator Γ1 Γ2 B) :=
-      fun Σ1 ζ1 ma s1 =>
-        outcome_map (fun '(MkDynMutResult ζ2 (MkMutResult a s2)) => MkDynMutResult ζ2 (MkMutResult (f _ (sub_comp ζ1 ζ2) a) s2)) (ma s1).
-    Definition dmut_bind {Γ1 Γ2 Γ3 A B Σ} (f : Mor Σ A (DynamicMutator Γ2 Γ3 B)) :
-      Mor Σ (DynamicMutator Γ1 Γ2 A) (DynamicMutator Γ1 Γ3 B) :=
-      fun Σ0 ζ0 m0 s0 =>
-        outcome_bind (m0 s0) (fun '(MkDynMutResult ζ1 (MkMutResult a s1)) =>
-        outcome_bind (f _ (sub_comp ζ0 ζ1) a s1) (fun '(MkDynMutResult ζ2 (MkMutResult b s2)) =>
-        outcome_pure (MkDynMutResult (sub_comp ζ1 ζ2) (MkMutResult b s2)))).
-    Definition dmut_join {Γ1 Γ2 Γ3 A Σ} :
-      Mor Σ (DynamicMutator Γ1 Γ2 (DynamicMutator Γ2 Γ3 A)) (DynamicMutator Γ1 Γ3 A) :=
-      fun Σ1 ζ1 => dmut_bind (fun _ _ m => m) ζ1.
-
-    Definition dmut_sub {A B Σ1 Σ2} (ζ2 : Sub Σ1 Σ2) : Mor Σ1 A B -> Mor Σ2 A B :=
-      fun m Σ3 ζ3 => m Σ3 (sub_comp ζ2 ζ3).
-    Global Arguments dmut_sub {_ _ _ _} ζ2 m.
-
-    Definition dmut_lift {Γ1 Γ2 A} {Σ} (m : Mutator Σ Γ1 Γ2 (A Σ)) : DynamicMutator Γ1 Γ2 A Σ :=
-      fun s => outcome_map (MkDynMutResult (sub_id Σ)) (m s).
-    Definition dmut_lift_kleisli {Γ1 Γ2 A B Σ} (m : A Σ -> Mutator Σ Γ1 Γ2 (B Σ)) :
-      A Σ -> DynamicMutator Γ1 Γ2 B Σ :=
-      fun a => dmut_lift (m a).
-    Definition dmut_fail {Γ1 Γ2 A Σ} (msg : string) : DynamicMutator Γ1 Γ2 A Σ :=
-      dmut_lift (mutator_fail msg).
-    Definition dmut_contradiction {Γ1 Γ2 A Σ} (msg : string) : DynamicMutator Γ1 Γ2 A Σ :=
-      dmut_lift (mutator_contradiction msg).
-    Definition dmut_block {Γ1 Γ2 A Σ} : DynamicMutator Γ1 Γ2 A Σ :=
-      dmut_lift (mutator_block).
-
-    Definition dmut_angelic {Γ1 Γ2 I A Σ} (ms : I -> DynamicMutator Γ1 Γ2 A Σ) : DynamicMutator Γ1 Γ2 A Σ :=
-      fun s1 => outcome_angelic (fun i => ms i s1).
-    Definition dmut_demonic {Γ1 Γ2 I A Σ} (ms : I -> DynamicMutator Γ1 Γ2 A Σ) : DynamicMutator Γ1 Γ2 A Σ :=
-      fun s1 => outcome_demonic (fun i => ms i s1).
-    Definition dmut_angelic_binary {Γ1 Γ2 A Σ} (m1 m2 : DynamicMutator Γ1 Γ2 A Σ) : DynamicMutator Γ1 Γ2 A Σ :=
-      dmut_angelic (fun b : bool => if b then m1 else m2).
-    Definition dmut_demonic_binary {Γ1 Γ2 A Σ} (m1 m2 : DynamicMutator Γ1 Γ2 A Σ) : DynamicMutator Γ1 Γ2 A Σ :=
-      dmut_demonic (fun b : bool => if b then m1 else m2).
-
-    Definition dmut_fresh {Γ A Σ} b (m : Mor (Σ ▻ b) Unit (DynamicMutator Γ Γ A)) :
-      Mor Σ Unit (DynamicMutator Γ Γ A) :=
-      fun Σ1 ζ1 _ s1 =>
-        outcome_map
-          (fun '(MkDynMutResult ζ r) =>
-             MkDynMutResult (sub_comp sub_wk1 ζ) r)
-          (m _ (sub_up1 ζ1) tt (wk1 s1)).
-    Global Arguments dmut_fresh {_ _ _} _ _.
-
-  End Proper.
 
   Module DynamicMutatorNotations.
 
@@ -1037,36 +540,56 @@ Module Mutators
   Import DynamicMutatorNotations.
   Local Open Scope dmut_scope.
 
-  (* Definition dmut_get {Γ Σ} : DynamicMutator Γ Γ (SymbolicState Γ) Σ := *)
-  (*   dmut_lift (fun _ _ => mutator_get). *)
-  (* Definition dmut_put {Γ Γ' Σ} (s : SymbolicState Γ' Σ) : DynamicMutator Γ Γ' Unit Σ := *)
-  (*   dmut_lift (fun _ ζ => mutator_put (subst ζ s)). *)
-  (* Definition dmut_modify {Γ Γ' Σ} (f : forall Σ', Sub Σ Σ' -> SymbolicState Γ Σ' -> SymbolicState Γ' Σ') : DynamicMutator Γ Γ' Unit Σ := *)
-  (*   dmut_lift (fun _ ζ => mutator_modify (f _ ζ)). *)
+  Definition dmut_state {Γ Γ' A Σ} (f : forall Σ', Sub Σ Σ' -> SymbolicState Γ Σ' -> A Σ' * SymbolicState Γ' Σ') :
+    DynamicMutator Γ Γ' A Σ :=
+    fun Σ1 ζ1 s1 =>
+      let (a, s2) := f Σ1 ζ1 s1 in
+      outcome_pure
+        {| dmutres_substitution := sub_id Σ1;
+           dmutres_result_value := a;
+           dmutres_result_state := s2;
+        |}.
+  Definition dmut_gets {Γ Σ A} (f : forall Σ1, Sub Σ Σ1 -> SymbolicState Γ Σ1 -> A Σ1) :
+    DynamicMutator Γ Γ A Σ :=
+    dmut_state (fun Σ1 ζ1 s1 => (f Σ1 ζ1 s1,s1)).
+  Definition dmut_get {Γ Σ} : DynamicMutator Γ Γ (SymbolicState Γ) Σ :=
+    dmut_gets (fun _ _ s => s).
+  Definition dmut_modify {Γ Γ' Σ} (f : forall Σ', Sub Σ Σ' -> SymbolicState Γ Σ' -> SymbolicState Γ' Σ') :
+    DynamicMutator Γ Γ' Unit Σ :=
+    dmut_state (fun Σ1 ζ1 s1 => (tt, f Σ1 ζ1 s1)).
+  Definition dmut_put {Γ Γ' Σ} (s : SymbolicState Γ' Σ) : DynamicMutator Γ Γ' Unit Σ :=
+    dmut_modify (fun Σ1 ζ1 _ => subst ζ1 s).
+
+  Definition dmut_state_local {Γ Γ' A Σ} (f : forall Σ', Sub Σ Σ' -> SymbolicLocalStore Γ Σ' -> A Σ' * SymbolicLocalStore Γ' Σ') :
+    DynamicMutator Γ Γ' A Σ :=
+    dmut_state (fun Σ1 ζ1 '(MkSymbolicState pc1 δ1 h1) => let (a, δ2) := f Σ1 ζ1 δ1 in (a,MkSymbolicState pc1 δ2 h1)).
+  Definition dmut_gets_local {Γ Σ A} (f : forall Σ1, Sub Σ Σ1 -> SymbolicLocalStore Γ Σ1 -> A Σ1) :
+    DynamicMutator Γ Γ A Σ :=
+    dmut_gets (fun Σ1 ζ1 s1 => f Σ1 ζ1 (symbolicstate_localstore s1)).
   Definition dmut_get_local {Γ Σ} : DynamicMutator Γ Γ (fun Σ => SymbolicLocalStore Γ Σ) Σ :=
-    dmut_lift (fun _ _ => mutator_get_local).
-  Definition dmut_put_local {Γ Γ' Σ} (δ' : SymbolicLocalStore Γ' Σ) : DynamicMutator Γ Γ' Unit Σ :=
-    dmut_lift (fun _ ζ => mutator_put_local (subst ζ δ')).
+    dmut_gets_local (fun _ _ δ => δ).
   Definition dmut_modify_local {Γ Γ' Σ} (f : forall Σ', Sub Σ Σ' -> SymbolicLocalStore Γ Σ' -> SymbolicLocalStore Γ' Σ') : DynamicMutator Γ Γ' Unit Σ :=
-    dmut_lift (fun _ ζ => mutator_modify_local (f _ ζ)).
+    dmut_state_local (fun Σ1 ζ1 δ1 => (tt,f Σ1 ζ1 δ1)).
+  Definition dmut_put_local {Γ Γ' Σ} (δ' : SymbolicLocalStore Γ' Σ) : DynamicMutator Γ Γ' Unit Σ :=
+    dmut_modify_local (fun Σ1 ζ1 _ => subst ζ1 δ').
   Definition dmut_pop_local {Γ x σ Σ} : DynamicMutator (Γ ▻ (x , σ)) Γ Unit Σ :=
-    dmut_lift (fun _ _ => mutator_pop_local).
+    dmut_modify_local (fun Σ1 ζ1 => env_tail).
   Definition dmut_pops_local {Γ} Δ {Σ} : DynamicMutator (Γ ▻▻ Δ) Γ Unit Σ :=
-    dmut_lift (fun _ _ => mutator_pops_local Δ).
+    dmut_modify_local (fun Σ1 ζ1 => env_drop Δ).
   Definition dmut_push_local {Γ x σ Σ} (t : Term Σ σ) : DynamicMutator Γ (Γ ▻ (x , σ)) Unit Σ :=
-    dmut_lift_kleisli mutator_push_local t.
+    dmut_modify_local (fun Σ1 ζ1 δ1 => env_snoc δ1 (x,σ) (subst (T:= fun Σ => Term Σ σ) ζ1 t)).
   Definition dmut_pushs_local {Γ Δ Σ} (δΔ : NamedEnv (Term Σ) Δ) : DynamicMutator Γ (Γ ▻▻ Δ) Unit Σ :=
-    dmut_lift (fun _ ζ => mutator_pushs_local (env_map (fun _ => sub_term ζ) δΔ)).
+    dmut_modify_local (fun Σ1 ζ1 δ1 => δ1 ►► subst (T := SymbolicLocalStore Δ) ζ1 δΔ).
   Definition dmut_get_heap {Γ Σ} : DynamicMutator Γ Γ SymbolicHeap Σ :=
-    dmut_lift (fun _ _ => mutator_get_heap).
-  (* Definition dmut_modify_heap {Γ Σ} (f : forall Σ', Sub Σ Σ' -> SymbolicHeap Σ' -> SymbolicHeap Σ') : DynamicMutator Γ Γ Unit Σ := *)
-  (*   dmut_lift (fun _ ζ => mutator_modify_heap (f _ ζ)). *)
-  (* Definition dmut_put_heap {Γ Σ} (h : SymbolicHeap Σ) : DynamicMutator Γ Γ Unit Σ := *)
-  (*   dmut_lift (fun _ ζ => mutator_put_heap (subst ζ h)). *)
+    dmut_state (fun _ _ s1 => (symbolicstate_heap s1,s1)).
+  Definition dmut_modify_heap {Γ Σ} (f : forall Σ', Sub Σ Σ' -> SymbolicHeap Σ' -> SymbolicHeap Σ') : DynamicMutator Γ Γ Unit Σ :=
+    dmut_modify (fun Σ1 ζ1 '(MkSymbolicState pc1 δ1 h1) => MkSymbolicState pc1 δ1 (f Σ1 ζ1 h1)).
+  Definition dmut_put_heap {Γ Σ} (h : SymbolicHeap Σ) : DynamicMutator Γ Γ Unit Σ :=
+    dmut_modify_heap (fun Σ1 ζ1 _ => subst ζ1 h).
   Definition dmut_eval_exp {Γ σ} (e : Exp Γ σ) {Σ} : DynamicMutator Γ Γ (fun Σ => Term Σ σ) Σ :=
-    dmut_lift (fun _ _ => mutator_eval_exp e).
+    dmut_gets_local (fun Σ1 ζ1 δ1 => symbolic_eval_exp δ1 e).
   Definition dmut_eval_exps {Γ Σ} {σs : Ctx (𝑿 * Ty)} (es : NamedEnv (Exp Γ) σs) : DynamicMutator Γ Γ (fun Σ => NamedEnv (Term Σ) σs) Σ :=
-    dmut_lift (fun _ _ => mutator_eval_exps es).
+    dmut_gets_local (fun Σ1 ζ1 δ1 => env_map (fun _ => symbolic_eval_exp δ1) es).
 
   Fixpoint dmut_freshen_tuplepat' {σs Δ} (p : TuplePat σs Δ) {Γ Σ} :
     DynamicMutator Γ Γ (fun Σ => Env (Term Σ) σs * NamedEnv (Term Σ) Δ)%type Σ :=
@@ -1133,13 +656,10 @@ Module Mutators
         | Some t =>
           let ζ := sub_single ςInΣ t in
           Some
-            {|
-              dmutres_context := Σ - (ς,σ);
-              dmutres_substitution := ζ;
-              dmutres_result :=
-                {| mutator_result_value := tt;
-                   mutator_result_state := subst ζ s;
-                |}
+            {| dmutres_context := Σ - (ς,σ);
+               dmutres_substitution := ζ;
+               dmutres_result_value := tt;
+               dmutres_result_state := subst ζ s;
             |}
         | None => None
         end
@@ -1160,18 +680,15 @@ Module Mutators
   (* Add the provided formula to the path condition. *)
   Definition dmut_assume_formula {Γ Σ} (fml : Formula Σ) : DynamicMutator Γ Γ Unit Σ :=
     fun Σ1 ζ1 s1 =>
-      let fml := sub_formula ζ1 fml in
+      let fml := subst ζ1 fml in
       match try_solve_formula fml with
       | Some true =>
         (* The formula is always true. Just skip it. *)
         outcome_pure
           {| dmutres_context := Σ1;
              dmutres_substitution := sub_id Σ1;
-             dmutres_result :=
-               {|
-                 mutator_result_value := tt;
-                 mutator_result_state := s1;
-               |}
+             dmutres_result_value := tt;
+             dmutres_result_state := s1;
           |}
       | Some false =>
         (* The formula is always false, so the path condition with it would become
@@ -1187,10 +704,8 @@ Module Mutators
                condition verbatim. *)
             {| dmutres_context := Σ1;
                dmutres_substitution := sub_id Σ1;
-               dmutres_result :=
-                 {| mutator_result_value := tt;
-                    mutator_result_state := symbolic_assume_formula fml s1;
-                 |}
+               dmutres_result_value := tt;
+               dmutres_result_state := symbolic_assume_formula fml s1;
             |}
           end
       end.
@@ -1200,20 +715,55 @@ Module Mutators
   Definition dmut_assume_exp {Γ Σ} (e : Exp Γ ty_bool) : DynamicMutator Γ Γ Unit Σ :=
     dmut_eval_exp e >>= fun _ _ => dmut_assume_term.
   Definition dmut_assume_prop {Γ Σ} (P : abstract_named Lit Σ Prop) : DynamicMutator Γ Γ Unit Σ :=
-    dmut_lift (fun _ ζ => mutator_assume_formula (formula_prop ζ P)).
+    dmut_assume_formula (formula_prop (sub_id Σ) P).
 
   Definition dmut_assert_formula {Γ Σ} (fml : Formula Σ) : DynamicMutator Γ Γ Unit Σ :=
-    dmut_lift_kleisli mutator_assert_formula fml.
+    fun (Σ1 : NCtx 𝑺 Ty) (ζ1 : Sub Σ Σ1) (s1 : SymbolicState Γ Σ1) =>
+      let fml1 := subst ζ1 fml in
+      match try_solve_formula fml1 with
+        | Some true =>
+          outcome_pure
+            {| dmutres_substitution := sub_id Σ1;
+               dmutres_result_value := tt;
+               dmutres_result_state := s1;
+            |}
+        | Some false =>
+          outcome_fail "Err [dmut_assert_formula]: unsatisfiable"
+        | None =>
+          (* Record the obligation. *)
+          outcome_assertk
+            (valid_obligation (obligation (symbolicstate_pathcondition s1) fml1))
+            (outcome_pure
+               (* We also want to assume the formula for the continuation, i.e.
+                  we actually perform a simple cut. First see if it's an
+                  equality that can be propagated. *)
+               match dmut_try_assume_eq s1 fml1 with
+               | Some r => r
+               | None =>
+                 (* We can't propagate the formula, so add it to the path
+                    condition. *)
+                 {| dmutres_substitution := sub_id Σ1;
+                    dmutres_result_value := tt;
+                    dmutres_result_state := symbolic_assume_formula fml1 s1;
+                 |}
+               end)
+        end%out.
+
   Definition dmut_assert_formulas {Γ Σ} (fmls : list (Formula Σ)) : DynamicMutator Γ Γ Unit Σ :=
-    dmut_lift_kleisli mutator_assert_formulas fmls.
+    fold_right (fun fml => dmut_bind_right (dmut_assert_formula fml)) (dmut_pure tt) fmls.
   Definition dmut_assert_term {Γ Σ} (t : Term Σ ty_bool) : DynamicMutator Γ Γ Unit Σ :=
     dmut_assert_formula (formula_bool t).
   Definition dmut_assert_exp {Γ Σ} (e : Exp Γ ty_bool) : DynamicMutator Γ Γ Unit Σ :=
-    dmut_lift (fun _ _ => mutator_assert_exp e).
+    dmut_eval_exp e >>= fun _ _ t => dmut_assert_term t.
   Definition dmut_produce_chunk {Γ Σ} (c : Chunk Σ) : DynamicMutator Γ Γ Unit Σ :=
-    dmut_lift_kleisli mutator_produce_chunk c.
+    dmut_modify_heap (fun _ ζ => cons (subst ζ c)).
   Definition dmut_consume_chunk {Γ Σ} (c : Chunk Σ) : DynamicMutator Γ Γ Unit Σ :=
-    dmut_lift_kleisli mutator_consume_chunk c.
+    dmut_get >>= fun Σ1 ζ1 '(MkSymbolicState pc1 δ1 h1) =>
+    dmut_angelic_list
+      "Err [dmut_consume_chunk]: empty extraction"
+      (List.map
+         (fun '(pc2 , h2) => (dmut_put {| symbolicstate_pathcondition := pc2; symbolicstate_localstore := δ1; symbolicstate_heap := h2 |}))
+         (extract_chunk_eqb (subst ζ1 c) h1 pc1)).
 
   Definition dmut_leakcheck {Γ Σ} : DynamicMutator Γ Γ Unit Σ :=
     dmut_get_heap >>= fun _ _ h =>
@@ -1261,9 +811,6 @@ Module Mutators
         ⨁ t : Term Σ τ =>
         dmut_sub (sub_snoc (sub_id _) (ς , τ) t) (dmut_consume a)
       end.
-
-    Definition dmut_consume' {Γ Σ} (asn : Assertion Σ) : DynamicMutator Γ Γ Unit Σ :=
-      dmut_lift (fun _ ζ => mutator_consume ζ asn).
 
     Definition dmut_call {Γ Δ τ Σr} (contract : SepContract Δ τ) (ts : NamedEnv (Term Σr) Δ) : DynamicMutator Γ Γ (fun Σ => Term Σ τ) Σr :=
       match contract with
@@ -1411,58 +958,76 @@ Module Mutators
 
     Section CallerContext.
 
-      Context {Σr : Ctx (𝑺 * Ty)} {Γ : Ctx (𝑿 * Ty)}.
+      Context {Γ : Ctx (𝑿 * Ty)}.
 
-      Definition dmut_consume_chunk_evar {Σe} (c : Chunk Σe) (L : EvarEnv Σe Σr) : DynamicMutator Γ Γ (EvarEnv Σe) Σr.
-      Proof.
-        apply dmut_lift.
-        intros Σ1 ζ1.
-        apply mutator_consume_chunk_evar.
-        exact c.
-        refine (env_map _ L).
-        intros ?.
-        apply option_map.
-        exact (sub_term ζ1).
-      Defined.
+      Definition dmut_consume_chunk_evar {Σe Σr} (c : Chunk Σe) (L : EvarEnv Σe Σr) : DynamicMutator Γ Γ (EvarEnv Σe) Σr :=
+        dmut_get_heap >>= fun _ ζ1 h =>
+        dmut_angelic_list
+          "Err [dmut_consume_chunk_evar]: empty extraction"
+          (List.map
+             (fun '(L', h') => dmut_put_heap h';; dmut_pure L')
+             (extract_chunk c h (subst ζ1 L))).
 
-      Definition dmut_consume_evar {Σe} (asn : Assertion Σe) (L : EvarEnv Σe Σr) : DynamicMutator Γ Γ (EvarEnv Σe) Σr.
-      Proof.
-        apply dmut_lift.
-        intros Σ1 ζ1.
-        apply mutator_consume_evar.
-        exact asn.
-        refine (env_map _ L).
-        intros ?.
-        apply option_map.
-        exact (sub_term ζ1).
-      Defined.
+      Fixpoint dmut_consume_evar {Σe Σr} (asn : Assertion Σe) (L : EvarEnv Σe Σr) : DynamicMutator Γ Γ (EvarEnv Σe) Σr :=
+        match asn with
+        | asn_bool b =>
+          match eval_term_evar L b with
+          | Some b' => dmut_assert_term b';; dmut_pure L
+          | None    => dmut_fail "Err [mutator_consume_evar]: uninstantiated variables when consuming bool assertion"
+          end
+        | asn_prop P =>
+          match evarenv_to_option_sub L with
+          | Some ζ => dmut_assert_formula (formula_prop ζ P);; dmut_pure L
+          | None   => dmut_fail "Err [mutator_consume_evar]: uninstantiated variables when consuming prop assertion"
+          end
+        | @asn_eq _ T t1 t2 =>
+          match eval_term_evar L t1, eval_term_evar L t2 with
+          | Some t1', Some t2' => dmut_assert_formula (formula_eq t1' t2') ;; dmut_pure L
+          | _       , _        => dmut_fail "Err [mutator_consume_evar]: uninstantiated variables when consuming equality assertion"
+          end
+        | asn_chunk c => dmut_consume_chunk_evar c L
+        | asn_if b a1 a2 =>
+          match eval_term_evar L b with
+          | Some b' => (dmut_assume_term b';; dmut_consume_evar a1 L)
+                         ⊗
+                       (dmut_assume_term (term_not b');; dmut_consume_evar a2 L)
+          | None    => dmut_fail "Err [mutator_consume_evar]: uninstantiated variables when consuming if assertion"
+          end
+        | asn_match_enum E k alts =>
+          match eval_term_evar L k with
+          | Some k1 =>
+            ⨁ k2 : 𝑬𝑲 E => dmut_assert_formula (formula_eq k1 (term_enum E k2));; dmut_consume_evar (alts k2) L
+          | None => dmut_fail "Err [mutator_consume_evar]: uninstantiated variables when consuming match enum assertion"
+          end
+        | asn_sep a1 a2 =>
+          dmut_consume_evar a1 L >>= fun _ _ => dmut_consume_evar a2
+        | asn_exist ς τ a =>
+          dmut_consume_evar a (L ► (ς∶τ ↦ None)) >>= fun _ _ La' =>
+          match env_unsnoc La' with
+          | (L' , Some _) => dmut_pure L'
+          | (L' , None)   => dmut_fail "Err [mutator_consume_evar]: uninstantiated existential variable"
+          end
+        end.
 
-      Definition dmut_assert_term_eq_evar {Σe σ} (te : Term Σe σ) (tr : Term Σr σ) (L : EvarEnv Σe Σr) : DynamicMutator Γ Γ (EvarEnv Σe) Σr.
-      Proof.
-        apply dmut_lift.
-        intros Σ1 ζ1.
-        apply (mutator_assert_term_eq_evar te (sub_term ζ1 tr)).
-        refine (env_map _ L).
-        intros ?.
-        apply option_map.
-        exact (sub_term ζ1).
-      Defined.
+      Definition dmut_assert_term_eq_evar {Σe Σr σ} (te : Term Σe σ) (tr : Term Σr σ) (L : EvarEnv Σe Σr) : DynamicMutator Γ Γ (EvarEnv Σe) Σr :=
+        (* Make sure we get the up to date substitution. *)
+        dmut_pure tt >>= fun Σr1 ζ1 _ =>
+        let tr1 := sub_term ζ1 tr in
+        let L1  := subst ζ1 L in
+        match match_term te tr1 L1 with
+        | Some e => dmut_pure e
+        | None => match eval_term_evar L1 te with
+                  | Some te1 => dmut_assert_formula (formula_eq te1 tr1);; dmut_pure L1
+                  | None => dmut_fail "Err [mutator_consume_evar]: uninstantiated existential variable"
+                  end
+        end.
 
-      Definition dmut_assert_namedenv_eq_evar {X Σe σs} (te : NamedEnv (X:=X) (Term Σe) σs) (tr : NamedEnv (Term Σr) σs) :
-        EvarEnv Σe Σr -> DynamicMutator Γ Γ (EvarEnv Σe) Σr.
-      Proof.
-        intros L.
-        apply dmut_lift.
-        intros Σ1 ζ1.
-        apply (mutator_assert_namedenv_eq_evar te).
-        refine (env_map _ tr).
-        intros ?.
-        exact (sub_term ζ1).
-        refine (env_map _ L).
-        intros ?.
-        apply option_map.
-        exact (sub_term ζ1).
-      Defined.
+      Equations(noeqns) dmut_assert_namedenv_eq_evar {X Σe Σr σs} (te : NamedEnv (X:=X) (Term Σe) σs) (tr : NamedEnv (Term Σr) σs) :
+        EvarEnv Σe Σr -> DynamicMutator Γ Γ (EvarEnv Σe) Σr :=
+        dmut_assert_namedenv_eq_evar env_nil env_nil := dmut_pure;
+        dmut_assert_namedenv_eq_evar (env_snoc E1 b1 t1) (env_snoc E2 b2 t2) :=
+          fun L => dmut_assert_namedenv_eq_evar E1 E2 L >>= fun _ ζ =>
+                   dmut_assert_term_eq_evar t1 (sub_term ζ t2).
 
     End CallerContext.
 
@@ -1476,6 +1041,9 @@ Module Mutators
          | None => dmut_fail "Err [dmut_call_evar]: uninstantiated variables after consuming precondition"
          end
       end.
+
+    (* TODO: The code should be rewritten so this variable can be removed. *)
+    Parameter dummy : 𝑺.
 
     Fixpoint dmut_exec_evar {Γ τ Σ} (s : Stm Γ τ) {struct s} :
       DynamicMutator Γ Γ (fun Σ => Term Σ τ) Σ :=
